src/Assembly/WithBedrock/SymbolicProofs.v
@@ -73,7 +73,8 @@ Section Memory.
 End Memory.
 
 
-Import BreakMatch DestructHead UniquePose.
+Require Import Crypto.Util.Prod.
+From Crypto.Util.Tactics Require Import BreakMatch DestructHead UniquePose.
 Import coqutil.Tactics.autoforward coqutil.Decidable coqutil.Tactics.Tactics.
 
 Local Coercion ExprRef : idx >-> expr.
@@ -491,8 +492,11 @@ Ltac step_GetReg :=
 Lemma Address_R s m (HR : R s m) sa o a s' (H : @Symbolic.Address sa o s = Success (a, s'))
   : R s' m /\ s :< s' /\ exists v, eval s' a v /\ @DenoteAddress sa m o = v.
 Proof using Type.
-  destruct o as [? ? ? ?]; cbv [Address DenoteAddress Syntax.mem_base_reg Syntax.mem_offset Syntax.mem_scale_reg] in *; repeat step_symex.
-  all : repeat first [ first [ step_symex | step_GetReg ]; try solve [repeat (eauto || econstructor)]; []
+  destruct o as [? ? ? ?]; cbv [Address DenoteAddress Syntax.mem_base_reg Syntax.mem_offset Syntax.mem_scale_reg err ret] in *; repeat step_symex.
+  all : repeat first [ progress inversion_ErrorT
+                     | progress inversion_pair
+                     | progress subst
+                     | first [ step_symex | step_GetReg ]; try solve [repeat (eauto || econstructor)]; []
                      | break_innermost_match_hyps_step; cbn [fst snd] in * ].
   all : Tactics.ssplit; eauto 99.
   all : eexists; split; eauto; [].
@@ -703,7 +707,7 @@ Lemma GetOperand_R s m (HR: R s m) so sa a i s'
   (H : @GetOperand so sa a s = Success (i, s'))
   : R s' m /\ s :< s' /\ exists v, eval s' i v /\ DenoteOperand sa so m a = Some v.
 Proof using Type.
-  cbv [GetOperand DenoteOperand] in *; BreakMatch.break_innermost_match.
+  cbv [GetOperand DenoteOperand err] in *; break_innermost_match; inversion_ErrorT.
   { eapply GetReg_R in H; intuition eauto. }
   { progress cbv [Load ret] in *.
     repeat (cbv [err] in *; cbn [fst snd] in * || step_symex || Tactics.destruct_one_match_hyp || inversion_ErrorT || Prod.inversion_prod || subst).
@@ -759,7 +763,7 @@ Lemma R_SetOperand s m (HR : R s m)
   v (Hv : eval s i v)
   : exists m', SetOperand sa sz m a v = Some m' /\ R s' m' /\ s :< s'.
 Proof using Type.
-  destruct a in *; cbn in H; [ | | solve [inversion H] ];
+  destruct a in *; cbn in H; cbv [err] in *; inversion_ErrorT; [ | ];
     cbv [SetOperand Crypto.Util.Option.bind SetReg64 update_reg_with Symbolic.update_reg_with] in *;
     repeat (BreakMatch.break_innermost_match_hyps; Prod.inversion_prod; ErrorT.inversion_ErrorT; subst).
 
@@ -886,10 +890,9 @@ Ltac destr_expr_beq :=
 Lemma standalone_operand_size_cases o n : standalone_operand_size o = Some n ->
   (n = 8 \/ n = 16 \/ n = 32 \/ n = 64)%N.
 Proof using Type.
-   destruct o; cbn.
+   destruct o; cbn; try congruence.
    { destruct r; cbn; inversion 1; subst; eauto. }
-   { destruct (mem_is_byte _); inversion 1; eauto. }
-   { inversion 1. }
+   { destruct (mem_bits_access_size _) as [ [] | ]; inversion 1; subst; eauto. }
 Qed.
 
 Lemma opcode_size_cases o n : opcode_size o = Some n ->
@@ -957,7 +960,7 @@ Proof using Type.
 Qed.
 
 Lemma operation_size_cases i n : Syntax.operation_size i = Some n ->
-  (((exists ls, i = Build_NormalInstruction Syntax.clc ls) /\ n = 1) \/ (n = 8 \/ n = 16 \/ n = 32 \/ n = 64))%N.
+  (((exists prefix ls, i = Build_NormalInstruction prefix Syntax.clc ls) /\ n = 1) \/ (n = 8 \/ n = 16 \/ n = 32 \/ n = 64))%N.
 Proof using Type.
   clear G.
   intuition idtac; DestructHead.destruct_head'_ex; subst; cbn in *.
@@ -1248,11 +1251,12 @@ Proof using Type.
   Unshelve. all : match goal with H : context[Syntax.adox] |- _ => idtac | _ => shelve end.
   { cbn [fold_right] in *; rewrite ?Z.bit0_odd, ?Z.add_0_r, ?Z.add_assoc in *; assumption. }
 
-  Unshelve. all : match goal with H : context[Syntax.cmovc] |- _ => idtac | _ => shelve end.
-  { (* cmovc *)
-    destruct vCF; cbn [negb Z.b2z Z.eqb] in *; eauto 9; [].
-    enough (m = m0) by (subst; eauto 9).
-    clear -Hm0 Hv frame G ; eauto using SetOperand_same. }
+  Unshelve. all : match goal with H : context[Syntax.cmovc] |- _ => idtac |  H : context[Syntax.cmovb] |- _ => idtac | _ => shelve end.
+  (* cmovc / cmovb *)
+  all: destruct vCF; cbn [negb Z.b2z Z.eqb] in *; eauto 9; [].
+  all: enough (m = m0) by (subst; eauto 9).
+  all: clear -Hm0 Hv frame G ; eauto using SetOperand_same.
+  all: fail.
 
   Unshelve. all : match goal with H : context[Syntax.cmovnz] |- _ => idtac | _ => shelve end.
   { (* cmovnz *)
@@ -1310,6 +1314,7 @@ Proof using Type.
              end; try eauto; try Lia.lia.
      destr (machine_flag_state m0); cbn [Tuple.tuple'] in *; DestructHead.destruct_head'_prod; subst; Prod.inversion_prod; subst.
      f_equal.
+     let E0 := match goal with H : rcrcnt _ _ = _ |- _ => H end in
      rewrite E0; cbn.
      rewrite <-2Z.bit0_odd, Z.lor_spec, Z.shiftl_spec_low, Bool.orb_false_r; trivial.
      pose_operation_size_cases; intuition (subst; cbn; clear; lia). }
